coq_translation/axiomatized/examples/generics/generics_new_type_idiom.v
@@ -4,28 +4,28 @@ Require Import CoqOfRust.CoqOfRust.
 Module Years.
   Unset Primitive Projections.
   Record t `{State.Trait} : Set := {
-    _ : i64;
+    x0 : i64;
   }.
   Global Set Primitive Projections.
   
-  Global Instance Get_0 : Notation.Dot 0 := {
-    Notation.dot '(Build_t x0) := x0;
+  Global Instance Get_0 `{State.Trait} : Notation.Dot "0" := {
+    Notation.dot x := let* x := M.read x in Pure x.(x0) : M _;
   }.
 End Years.
-Definition Years := @Years.t.
+Definition Years `{State.Trait} : Set := M.val Years.t.
 
 Module Days.
   Unset Primitive Projections.
   Record t `{State.Trait} : Set := {
-    _ : i64;
+    x0 : i64;
   }.
   Global Set Primitive Projections.
   
-  Global Instance Get_0 : Notation.Dot 0 := {
-    Notation.dot '(Build_t x0) := x0;
+  Global Instance Get_0 `{State.Trait} : Notation.Dot "0" := {
+    Notation.dot x := let* x := M.read x in Pure x.(x0) : M _;
   }.
 End Days.
-Definition Days := @Days.t.
+Definition Days `{State.Trait} : Set := M.val Days.t.
 
 Module Impl_generics_new_type_idiom_Years.
   Definition Self := generics_new_type_idiom.Years.
