coq_translation/axiomatized/examples/hello_world/formatted_print.v
@@ -7,12 +7,12 @@ Parameter main : forall `{State.Trait}, M unit.
 Module Structure.
   Unset Primitive Projections.
   Record t `{State.Trait} : Set := {
-    _ : i32;
+    x0 : i32;
   }.
   Global Set Primitive Projections.
   
-  Global Instance Get_0 : Notation.Dot 0 := {
-    Notation.dot '(Build_t x0) := x0;
+  Global Instance Get_0 `{State.Trait} : Notation.Dot "0" := {
+    Notation.dot x := let* x := M.read x in Pure x.(x0) : M _;
   }.
 End Structure.
-Definition Structure := @Structure.t.
+Definition Structure `{State.Trait} : Set := M.val Structure.t.
