coq_translation/axiomatized/examples/scoping_rules/scoping_rules_lifetimes_bounds.v
@@ -6,16 +6,16 @@ Module Ref.
     Context {T : Set}.
     Unset Primitive Projections.
     Record t `{State.Trait} : Set := {
-      _ : ref T;
+      x0 : ref T;
     }.
     Global Set Primitive Projections.
     
-    Global Instance Get_0 : Notation.Dot 0 := {
-      Notation.dot '(Build_t x0) := x0;
+    Global Instance Get_0 `{State.Trait} : Notation.Dot "0" := {
+      Notation.dot x := let* x := M.read x in Pure x.(x0) : M _;
     }.
   End Ref.
 End Ref.
-Definition Ref := @Ref.t.
+Definition Ref `{State.Trait} : Set := M.val Ref.t.
 
 Module Impl_core_fmt_Debug_for_scoping_rules_lifetimes_bounds_Ref_T.
   Section Impl_core_fmt_Debug_for_scoping_rules_lifetimes_bounds_Ref_T.
